more writing

examples/algorithms/IntervalIntersect.fst
@@ -45,6 +45,7 @@ type offset = int
 /// As in its Haskell version, I represent intervals as a datatype constructor.
 ///  Note that [from] is inclusive and [to] is not inclusive.
 type interval = | I: from:offset -> to:offset -> interval
+
 /// F* automatically generates accessor functions for the named arguments of the
 /// dependently typed constructor. Given [i:interval], [I?.from i] returns the
 /// start of the interval. Datatypes with a single constructor, also allow for
@@ -52,12 +53,20 @@ type interval = | I: from:offset -> to:offset -> interval
 /// alternative to records.
 ///
 /// We define the goodness of [interval list]s in the same way as Joachim did in
-/// Coq. A [good interval list] is ordered and consists of non-empty intervals.
-/// 
+/// Coq. A [good interval list] is ordered and consists of non-empty disjoint
+/// intervals.
+
 let rec goodLIs (is:list interval) (lb:offset) =
   match is with
   | [] -> true
   | I f t :: is -> lb <= f && f < t && goodLIs is t
+
+/// Contrary to Joachim's informal claims, already in his Coq development
+/// intervals are however not necessarily non-adjacent. This is a good example
+/// for a divergence between formal spec and human intuitive expectations. Just
+/// because we verified something, doesn't necessarily mean that we get what we
+/// want. Something has to give, either we remove the informal non-adjacency
+/// requirement, or strengthen the [goodLIs] predicate to require [lb < f].
 
 let good is =
   match is with
@@ -70,9 +79,9 @@ let good is =
 /// types, to add the requirement to the [intervals].
 let intervals = is:list interval{good is}
 
-/// This is a first example of how F* closely intertwines programming and
-/// verification. Often Z3 can prove refinements automatically by discharging
-/// them as SMT constraint queries.
+/// This is a first example for F*'s closely intertwines programming and
+/// verification style. Often Z3 can prove refinements automatically by
+/// discharging them as SMT constraint queries.
 
 /// The following function is needed in the termination argument for the
 /// [intersect] function. I will get back to it in a bit.
@@ -99,9 +108,9 @@ private let rec go (is1 is2:intervals)
   : Pure intervals
          (requires True)
          (ensures (fun ris ->
-           ( is1=[] \/ is2=[] ==> ris=[])
-         /\ ( Cons? is1 /\ Cons? is1 /\ Cons? ris  ==> 
-             (hd ris).from >= max (hd is1).from (hd is2).from  )
+          ( is1=[] \/ is2=[] ==> ris=[])
+        /\ ( Cons? is1 /\ Cons? is1 /\ Cons? ris  ==>
+            (hd ris).from >= max (hd is1).from (hd is2).from  )
          ))
          (decreases %[List.length is1 + List.length is2; needs_reorder is1 is2]) =
 /// The termination argument uses the lexicographic ordering of two values: the
@@ -122,7 +131,7 @@ private let rec go (is1 is2:intervals)
       // subset
       else if i1.to = i2.to then I f' (I?.to i1) :: go is1 is2
       // overlapping
-      else  I f' (i2.to) ::
+      else I f' (i2.to) ::
         go (I (i2.to) (i1.to) :: is1) is2
     end
 
@@ -140,7 +149,13 @@ let intersect (is1 is2:intervals) =
 /// Z3 to complete the proof? As Arthur C. Clark famously said: Any sufficiently
 /// advanced technology is indistinguishable from magic.
 ///
-/// Proof by induction. good is
+/// I am cryptographer and we like to give paper proofs of results that seem
+/// almost magical. Naturally, the proof is by induction. So after a recursive
+/// call to [go], the induction hypothesis is available, and we know that the
+/// returned [intervals] are good. The SMT solver can also prove locally that
+/// the interval prepended to this result is non-empty, what remains to be shown
+/// is that together they are ordered. That is where knowing that the [from] of
+/// the first result intervals is the [max] saves the day.
 
 (**** Proving functional correctness *)
 
@@ -148,25 +163,51 @@ let intersect (is1 is2:intervals) =
 /// are few blemishes, like the F* bug with local functions that I discovered, or
 /// the low priority given to a weakes precondition calculus supporting [when]
 /// clauses, but overall I was positively surprised by the speed at which I
-/// could translate the Haskell and Coq code to F* and with how little I had to
-/// do in terms of proofs.
+/// could translate the Haskell and Coq code to F* and by how little I had to
+/// do in terms of writing proofs.
 
 /// Mindful of Clarke's second law that the only way of discovering the limits
 /// of the possible is to venture a little way past them into the impossible, we
 /// wont stop when its easy. The second property that Joachim proved about the
 /// [intersect] function is that it corresponds to its corresponding function.
 /// This sounds a bit tautological. What is meant here is that it corresponds to
-/// another way of representing intervals and implementing intersection, that
-/// ideally is in some sense more pure and mathematical.
+/// another way of representing intervals and another way of implementing
+/// intersection in that representation. Ideally this alternative way should in
+/// some sense be more pure and mathematical.
 ///
-/// The natural way to represent intervals is of course as sets, and interval
-/// intersection then simply becomes set intersection. The FStar.Set module provides pure and total 
+(***** The mathematical representation of intervals *)
+///
+/// In traditional mathematics intervals are of course represented as sets, and
+/// interval intersection then simply becomes set intersection. Luckily, the
+/// [FStar.Set] module already provides us with set operations proven to be pure
+/// and total.
+///
+/// However, unlike `Coq.Sets.Ensembles` the representation of [set a] as a
+/// function [a -> bool] is abstract in F*. Consequently, we cannot define
+/// [range] using a lambda expression. This is what is lost, but what is gained
+/// by hiding the representation. We can change the way sets are represented in
+/// [FStar.Set] under the hood, without affecting users of the library. Indeed
+/// F* libraries often have two implementations, one acting as a model to prove
+/// that the pre- and post-conditions of the API do not allow to prove [False],
+/// and an actual implementation for running the actual program. In fact different
+/// extraction targets, such as OCaml and F# would typically provide different
+/// implementations, e.g. the OCaml implementation is based on
+/// [Batteries|http://batteries.forge.ocamlcore.org/].
 
-let rangeGT (f t:offset): GTot (Set.set offset)
-  =
-  Set.intension (fun z -> f <= z && z < t)
+/// The declarative definition of a set using a predicate that all set members
+/// need to satisfy is known in mathematics as an intensional definition.
+/// Certain sets, for example the set of even numbers can only be defined
+/// intensionally. My intuition is that intensional definitions are more concise and better suited for proof, conversely, extensional definitions are more explicit guaranteeing that sets are finite.
+///
+/// To get the best of both worlds, I give both an intensional and an
+/// extensional description of integer ranges, but make the intensional
+/// definition ghost. This means that it never has to be extracted to [BatSet]
+/// based OCaml code.
+let rangeGT (f t:offset): GTot (Set.set offset) = Set.intension (fun z -> f <= z &&
+  z < t)
 
-
+/// I use the ghostly intensional definition to specify the logical properties
+/// of the extensional definition.
 let rec range (f t:offset): Tot (r:Set.set offset{r==rangeGT f t})
   (decreases %[t-f])
   =
@@ -178,6 +219,13 @@ let rec range (f t:offset): Tot (r:Set.set offset{r==rangeGT f t})
     Set.union (Set.singleton f) ( range (f+1) t )
   )
 
+/// The proof that the extensionally defined set is the same as the
+/// intensionally defined set uses induction, and the set equality `[f,t] = {f}
+/// u [f+1,t]`.
+
+/// Using [range] and following the Coq code, the [semI] and [sem] functions
+/// define the semantic of bounds based interval representations in terms of
+/// integer sets.
 let semI (i : interval) : Set.set offset =
   range i.from i.to
 
@@ -186,6 +234,13 @@ let rec sem (is : intervals) : Set.set offset =
   | [] -> Set.empty
   | (i :: is) -> Set.union (semI i) (sem is)
 
+/// This simple lemma should likely move to the [FStar.Set], but it gives me the
+/// opportunity explain some of F* automation power. The body of the lemma is
+/// straightforward and the proof is by definition. What the SMT pattern lemma
+/// does is to 'remind' the SMT solver that it can prove disjointness whenever
+/// the intersection of two sets is empty. Below I commented out two invocations
+/// of the lemma where the lemma is now automatically applied because of the
+/// pattern.
 let lemma_disjoint_intro (#a:eqtype) (s1 s2:Set.set a)
   : Lemma
     (requires Set.equal (Set.intersect s1 s2) Set.empty)
@@ -193,88 +248,146 @@ let lemma_disjoint_intro (#a:eqtype) (s1 s2:Set.set a)
     [SMTPat (Set.disjoint s1 s2)]
  = ()
 
-/// The following lemma is inspired by Joachim's
-/// `Intersection_range_semLIs_empty` lemma. It expresses the same idea and is
-/// proven by induction on an increasing lower bound.
-let rec lemma_semI_sem_disjoint (i:interval) (is:intervals) (lb:offset)
+
+/// I use the lemma to prove that an interval is disjoint from an interval list
+/// whenever their concatenaton is [good].
+let lemma_semI_sem_disjoint (i:interval) (is:intervals)
   : Lemma
-    (requires goodLIs is lb /\ i.to <= lb)
-    (ensures Set.disjoint (semI i) (sem is))
+    (requires good (i::is))
+    (ensures (Set.disjoint (semI i) (sem is)))
   =
-  if (Cons? is) then
-      lemma_semI_sem_disjoint i (tl is) (hd is).to
-  else ();
-  Set.lemma_equal_elim (Set.intersect (semI i) (sem is)) Set.empty
+///  The following local lemma is inspired by Joachim's
+///  `Intersection_range_semLIs_empty` lemma. It expresses the same idea and is
+///  proven by induction on an increasing lower bound.
+  let rec lemma_semI_sem_lb_disjoint (i:interval) (is:intervals) (lb:offset)
+    : Lemma
+      (requires goodLIs is lb /\ i.to <= lb)
+      (ensures Set.disjoint (semI i) (sem is))
+    =
+    if (Cons? is) then
+       lemma_semI_sem_lb_disjoint i (tl is) (hd is).to
+    else ();
+    Set.lemma_equal_elim (Set.intersect (semI i) (sem is)) Set.empty in
+///
+  lemma_semI_sem_lb_disjoint i is i.to
+  // ; lemma_disjoint_intro (semI h) (sem t) //needed if SMTPat is removed
 
-/// I use the lemma to prove that the head of an interval list is disjoint from
-/// the tail of the interval list.
+(***** The heart of the proof *)
 
-let lemma_intervals_disjoint (is:intervals{Cons? is})
-  : Lemma
-    (ensures (Set.disjoint (semI (hd is)) (sem (tl is))))
-  =
-  let h::t = is in
-  if (Cons? t) then (
-    lemma_semI_sem_disjoint h t h.to
-  ) else ()
+/// We now get into the heart of the correctness proof for [intersect]. Recall that Joachim's algorithm (after switching) distinguishes three cases about the head elements of two interval lists:
+///  1. the heads are disjoint
+///  2. the second head is a subset of the first
+///  3. the tho heads are overlapping
+/// We prove a lemma for each case.
 
-
+/// The first lemma states that if the heads are disjoint, then the head with
+/// the smaller [to] can be dropped from the [intersect] computation.
 let lemma_disjoint_prefix (is1:intervals{Cons? is1})  (is2:intervals{Cons? is2})
   : Lemma
     (requires (hd is1).from >= (hd is2).to )
     (ensures (Set.intersect (sem is1) (sem is2) == Set.intersect (sem (is1)) (sem (tl is2))))
   =
   let h2 = hd is2 in
-  lemma_intervals_disjoint (h2::is1);
+  lemma_semI_sem_disjoint h2 is1;
   Set.lemma_equal_elim (Set.intersect (sem is1) (sem is2)) (Set.intersect (sem (is1)) (sem (tl is2)))
 
+/// The second lemma states that if the second head is a subset of the first,
+/// then the result of [intersect] is the union of that subset and the
+/// [intersect] computation with both heads dropped.
+let lemma_subset_prefix (is1:intervals{Cons? is1}) (is2:intervals{Cons? is2})
+  : Lemma
+    (requires (hd is1).to = (hd is2).to /\ (hd is1).from < (hd is2).to)
+    (ensures (
+      let h1::t1, h2::t2 = is1,is2 in
+      let f' = max h1.from h2.from in
+      Set.intersect (sem is1) (sem is2) ==
+      Set.union (semI (I f' h2.to))
+                (Set.intersect ( sem t1)
+                               ( sem t2)) ))
+  =
+  let h1::t1,h2::t2 = is1, is2 in
+  let f' = max h1.from h2.from in
+  lemma_semI_sem_disjoint h2 t1;
+  lemma_semI_sem_disjoint h1 t2;
+  Set.lemma_equal_elim (Set.intersect (sem is1) (sem is2))
+                       (Set.union (semI (I f' h2.to))
+                                  (Set.intersect ( sem t1)
+                                                 ( sem t2)) )
+
+/// This is the hardest of the three cases and we ramp up the SMT solvers
+/// timeout to prove it.
 #set-options "--z3rlimit 15"
+
+/// No, unfortunately this is not a panacea. Rather, it is a proven recipe for
+/// spending too much time idlying just to get the infamous "(Error) could not
+/// prove post-condition" error. Time that one should instead spend on thinking
+/// about the nature of what needs to be proven.
+///
+/// To shortcut the thinking a bit, I looked at the Coq proof script. While most
+/// of it was pretty well obfuscated without a detailed knowledge of Coq tactics
+/// and the ability to see the proof state, it revealed some crucial hints.
+///
+/// One was the equivalent of the [lemma_semI_sem_lb_disjoint] lemma and its
+/// proof. The other was the importance of set operatoin distributivity for the
+/// proof.
 let rec lemma_overlapping_prefix (is1:intervals{Cons? is1}) (is2:intervals{Cons? is2})
   : Lemma
     (requires (hd is1).to > (hd is2).to /\ (hd is1).from < (hd is2).to)
     (ensures (
-        let h1::t1 = is1 in let h2::t2 = is2 in
-        let f' = max h1.from h2.from in
-        Set.intersect (sem is1) (sem is2) ==
-        Set.union (semI (I f' h2.to))
-                  (Set.intersect (Set.union (range (h2.to) (h1.to)) (sem t1))
-                                 (sem t2)) ))
+      let h1::t1 = is1 in let h2::t2 = is2 in
+      let f' = max h1.from h2.from in
+       Set.intersect (sem is1) (sem is2) ==
+      Set.union (semI (I f' h2.to))
+                (Set.intersect (Set.union (range (h2.to) (h1.to)) (sem t1))
+                               (sem t2)) ))
   =
   let h1::t1 = is1 in
   let h2::t2 = is2 in
   let f' = max h1.from h2.from in
+/// The [assert] below expresses the outcome of the repeated application of set
+/// distributive law to state the following equality:
+///
 /// (h1 u t1) n (h2 u t2) = (h1 n (h2 u t2)) u (t1 n (h2 u t2))
-///                         = (h1 n h2) u (h1 n t2) u (t1 n h2) u (t1 n t2)
+///                       = (h1 n h2) u (h1 n t2) u (t1 n h2) u (t1 n t2)
+///
   let is1_n_is2 = Set.intersect (sem is1) (sem is2) in
   assert (Set.equal is1_n_is2
                     (Set.union (Set.union (Set.intersect (semI h1) (semI h2))
                                           (Set.intersect (semI h1) (sem t2)))
                                (Set.union (Set.intersect (semI h2) (sem t1))
                                           (Set.intersect (sem t1) (sem t2)))));
-///  h1 n h2 = [f', h2.to]
+///
+///  The rest of the proof simplifies the first three of the four intersects:
+///  1. h1 n h2 = [f', h2.to]
   assert (Set.equal (Set.intersect (semI h1) (semI h2)) (semI (I f' h2.to)));
-///  h1 n t2 = [h2.to h1.to] n t2
-  lemma_semI_sem_disjoint (I h1.from h2.to) t2 h2.to;
-  Set.lemma_equal_elim (range h1.from h1.to)
-                       (Set.union (range h1.from h2.to) (range h2.to h1.to));
-  Set.lemma_equal_elim (Set.intersect (range h1.from h1.to) (sem t2))
-                       (Set.intersect (range h2.to h1.to) (sem t2));
-///  h2 n t1 = empty
-  lemma_intervals_disjoint (h2::t1);
+///  2. h1 n t2 = [h2.to h1.to] n t2
+  lemma_semI_sem_disjoint (I h1.from h2.to) t2;
+  assert (Set.equal (range h1.from h1.to)
+                    (Set.union (range h1.from h2.to) (range h2.to h1.to)));
+  assert (Set.equal (Set.intersect (range h1.from h1.to) (sem t2))
+                    (Set.intersect (range h2.to h1.to) (sem t2)));
+///  3. h2 n t1 = empty
+  lemma_semI_sem_disjoint h2 t1;
+///
+/// The proof now applies the distributive law in the other direction to combine the 3rd and 4th intersect:
   Set.lemma_equal_elim is1_n_is2
                        (Set.union (semI (I f' h2.to))
                                   (Set.intersect (Set.union (range (h2.to) (h1.to))
                                                             (sem t1))
                                                  (sem t2)) )
 
+/// The following pragma resets the SMT solver to its original resource limit (roughly 5 seconds):
 #reset-options
+
+/// The final proof is by case analysis, in each step relying on the induction
+/// hypothesis and one of the lemmas. Again the [assert]s document document the
+/// proof.
 let rec lemma_intersection_spec (is1:intervals) (is2:intervals)
   : Lemma
     (ensures (Set.equal ( sem (intersect is1 is2) ) (Set.intersect (sem is1) (sem is2))))
     (decreases %[List.length is1 + List.length is2; needs_reorder is1 is2])
   =
   match is1, is2 with
-  | [], [] -> ()
   | _, [] -> ()
   | [], _ -> ()
   | i1::is1, i2::is2 ->
@@ -282,25 +395,34 @@ let rec lemma_intersection_spec (is1:intervals) (is2:intervals)
        let f' = max (i1.from) (i2.from) in
        // reorder for symmetry
        if i1.to < i2.to then lemma_intersection_spec (i2::is2) (i1::is1)
-       // disjoint i2.from i2.to, i1.from, i1.to
+       // disjoint: i2.from < i2.to <= i1.from < i1.to
        else if i1.from >= i2.to then (
-         lemma_intersection_spec (i1::is1) is2;
+         // lemma_disjoint_intro (semI i1) (semI i2); //needed if SMTPat is removed
          assert (Set.disjoint (semI i1) (semI i2));
+         lemma_intersection_spec (i1::is1) is2;
          lemma_disjoint_prefix (i1::is1) (i2::is2)
        )
-       // subset min (i1.from) (i2.from), f', i1.to=i1.to,
+       // subset: min (i1.from) (i2.from) <= f' <= i1.to=i2.to,
        else if i1.to = i2.to then (
          assert (Set.equal (Set.intersect (semI i1) (semI i2)) (semI (I f' i1.to)));
-         lemma_intervals_disjoint (i2::is1);
-         lemma_intervals_disjoint (i1::is2);
-         lemma_intersection_spec is1 is2
+         lemma_intersection_spec is1 is2;
+         lemma_subset_prefix (i1::is1) (i2::is2)
        )
-       // overlapping
+       // overlapping: min (i1.from) (i2.from) <= f' <= i2.to < i1.to
        else  (
-         lemma_overlapping_prefix (i1::is1) (i2::is2);
-         lemma_intersection_spec (I (i2.to) (i1.to) :: is1) is2
+         lemma_intersection_spec (I (i2.to) (i1.to) :: is1) is2;
+         lemma_overlapping_prefix (i1::is1) (i2::is2)
        )
     end
+
+(***** Taking stock *)
+
+/// Clearly this second part of the verification of [intersect] was much harder.
+/// While in the first part we used F* essentially as a programming language
+/// with stronger types and great automation, here we relied in a fundamental
+/// way on hand written lemmas and proofs.
+///
+/// 
 
 /// A simple print and test function confirme the code can be executed.
 open FStar.All
@@ -319,11 +441,10 @@ let ppInterval (I f t) = sprintf "0x%d-0x%d" f t
 let ppIntervals is = FStar.List.fold_left (sprintf "%s %s") "" (FStar.List.map ppInterval is)
 let main = stdout <| ppIntervals (intersect [I 3 10; I 10 15] [I 1 4; I 10 14])
 
-/// sorted, non-empty, disjoint and non-adjacent
 
 (***** Why functional programming and types *)
 
-/// Today there are many areas in which bugs in programs have become so
+/// There are many areas in which bugs in programs have become so
 /// expensive, that programmers are willing to walk an extra mile to avoid bug
 /// infested code.
 ///
@@ -331,15 +452,17 @@ let main = stdout <| ppIntervals (intersect [I 3 10; I 10 15] [I 1 4; I 10 14])
 /// and program verification.
 ///
 /// There are some similarities and synergies between the two. Modern languages,
-/// such as strictly typed functional programming languages, make (mathematical)
-/// reasoning about program code easier and thus potentially make program
-/// verification easier. There are also differences, the expressivity of a
-/// programming language helps programmers understand their programs, but
-/// supporting all that in a verification tool may hinder automation and may
-/// result in a large trusted computing base. The established wisdom here is to
-/// have a core calculus that is as small as possible, and to translate the more
-/// complex human readable code to that calculus.
+/// such as strictly typed functional programming languages, ease (mathematical)
+/// reasoning about programs and program verification. There are also
+/// differences, the expressivity and multiple levels of abstraction offered by
+/// a programming language like Haskell make the code more readable,
+/// but supporting these in a verification tool may get in the way of automation
+/// and may result in a large trusted computing base. The established wisdom
+/// here is to have a core calculus that is as small as possible, and to
+/// translate the more complex human readable code to that calculus.
 
 (***** Efforts and gains *)
 
-/// test
+/// I am not a big fan of filling in time sheets. I might try Joachim's tool one day to do a self study on the effects of (self)-surveillance on my productivity.
+///
+/// When a distinguished but elderly scientist states that something is possible, they are almost certainly right. When they state that something is impossible, they are very probably wrong.
